coq/two/LambdaTwoNI.v
@@ -1,3 +1,4 @@
+Require Import Program.Tactics.
 Require Import MyTactics.
 Require Import LabelAlgebra.
 Require Import LambdaTwo.
@@ -8,7 +9,12 @@ Set Implicit Arguments.
 
 Section NI.
 
-Context (lab : two) (P : value -> value -> Prop).
+Context (lab : two)
+        (P : value -> value -> Prop)
+        (Prefl : forall x, P x x)
+        (Psym : forall x y, P x y -> P y x)
+        (Ptrans : forall x y z, P x y -> P y z -> P x z)
+        (Pv : forall v1 v2, value_Lequiv lab P v1 v2 -> P v1 v2).
   
 (** * Preliminary lemmas. *)
 (** ** The pc label is below the label of the resulting atom. *)
@@ -17,19 +23,117 @@ Lemma eval_pc_lower_bound :
     pc; e ⊢ t ⇓ Atom v l ->
     pc ⊑ l.
 Proof.
-  Admitted.
+  intros pc e t v l Heval.
+  remember (Atom v l) as a.
+  generalize dependent l. generalize dependent v.
+  induction Heval; intros v' l' Heq; inversion Heq; subst; auto.
+  destruct l; destruct pc; reflexivity.
+  transitivity l1. 
+    apply (IHHeval1 (VClos e1' t1') l1). reflexivity.
+    apply (IHHeval3 v' l'). reflexivity.
+Qed.
+
+Lemma join_top :
+  forall l, l ⊔ Top2 = Top2.
+Proof. destruct l; reflexivity. Qed.
+
+Lemma join_bot :
+  forall l, l ⊔ Bottom2 = l.
+Proof. destruct l; reflexivity. Qed.
+
+Lemma atom_Lequiv_raise_bot :
+  forall v1 v2,
+    atom_Lequiv Bottom2 P (Atom v1 Bottom2) (Atom v2 Bottom2) ->
+    atom_Lequiv Bottom2 P (Atom v1 Top2) (Atom v2 Top2).
+Proof.
+  intros. left. repeat (split; auto). apply Pv.
+  destruct lab.
+    inversion H.
+      destruct_conjs. inversion H2.
+      inversion H0.
+        unfold value_Lequiv. destruct_conjs. auto.
+        destruct_conjs. inversion H1.
+    Admitted.
+        
+
+Lemma atom_Lequiv_raise_top :
+  forall v1 v2,
+    atom_Lequiv Top2 P (Atom v1 Bottom2) (Atom v2 Bottom2) ->
+    atom_Lequiv Top2 P (Atom v1 Top2) (Atom v2 Top2).
+Proof.
+  intros. destruct v1; destruct v2.
+  inversion H.
+    destruct_conjs. inversion H0.
+    inversion H0; destruct_conjs. 
+      inversion H1.
+      right. right. auto.
+    inversion H.
+      destruct_conjs. inversion H0.
+      inversion H0; destruct_conjs.
+        inversion H1.
+        inversion H3.
+    inversion H.
+      destruct_conjs. inversion H0.
+      inversion H0; destruct_conjs.
+        inversion H1.
+        inversion H3.
+    inversion H.
+      destruct_conjs. inversion H0.
+      inversion H0; destruct_conjs.
+        inversion H1.
+        right. right. auto.
+Qed.
 
 (** ** Strong version of the non-interference theorem. *)
 Lemma NI_strong :
   forall pc1 pc2 e1 e2 t1 t2 a1 a2,
-    pc1 =L pc2 ->
+    pc1 = pc2 ->
     env_Lequiv lab P e1 e2 ->
     term_equiv t1 t2 ->
     pc1; e1 ⊢ t1 ⇓ a1 ->
     pc2; e2 ⊢ t2 ⇓ a2 ->
     atom_Lequiv lab P a1 a2.
 Proof.
-  Admitted.
+  intros pc1 pc2 e1 e2 t1 t2 a1 a2 Hpc He Ht Heval.
+  generalize dependent a2.
+  generalize dependent t2.
+  generalize dependent e2.
+  generalize dependent pc2.
+  induction Heval;
+    intros pc2 Hpc e2 He t2' Ht a2' Heval2'; destruct t2'; try inversion Ht.
+    (* Eval_nat *)
+    inversion Heval2'. subst.
+    destruct lab; destruct pc2.
+      right. left. auto.
+      left. auto.
+      right. right. auto.
+      right. right. auto.
+    (* Eval_var *)
+    inversion Heval2'. subst. unfold env_Lequiv in He.
+    assert (atom_Lequiv lab P (Atom v l) (Atom v0 l0)) by
+        (eapply list_forall2_atIndex; eassumption).
+    assert (l = l0) by
+        (eapply atom_Lequiv_lab_inv; eassumption).
+    subst.
+    destruct lab; destruct pc2;
+      try (rewrite join_bot; assumption);
+      try (rewrite join_top; destruct l0; [
+             try apply atom_Lequiv_raise_bot;
+             try apply atom_Lequiv_raise_top; assumption
+           | assumption ]).
+    (* Eval_lam *)
+    inversion Heval2'. subst.
+    destruct lab; destruct pc2.
+      right. left. auto.
+      assert (P (VClos e t) (VClos e2 t2')).
+          apply Pv. unfold value_Lequiv. auto.
+        left. auto.
+      assert (P (VClos e t) (VClos e2 t2')).
+          apply Pv. unfold value_Lequiv. auto.
+        right. right. auto.
+      right. right. auto.
+    (* Eval_app *)
+    Admitted.
 
 (** * General non-interference theorem. *)
 Theorem general_non_interference :
